WIP

tests/lean/run/mvcgenTick.lean
@@ -1,58 +1,21 @@
 module
 
-public import Std.Do.Triple.Basic
-import Std.Tactic.Do
+public structure State where
+  private count : Nat
 
-open Std.Do
-
-public section
-
-structure TickM.State where
-  count : Nat
-
-@[expose] def TickM (α : Type) := StateM TickM.State α
-
-namespace TickM
-
-instance : Monad TickM := inferInstanceAs (Monad (StateM TickM.State))
-instance : LawfulMonad TickM := inferInstanceAs (LawfulMonad (StateM TickM.State))
-
--- Is this what we want?
-instance : Std.Do.WP TickM (.arg TickM.State .pure) := inferInstanceAs (Std.Do.WP (StateM TickM.State) _)
-
-def run (m : TickM α) : α := (StateT.run m ⟨0⟩).1
-def tick : TickM Unit := modify (m := StateM _) (fun s => ⟨s.count + 1⟩)
-def tick' : TickM Unit := fun s => ⟨(), ⟨s.count + 1⟩⟩
-
-def checkBound (n : Nat) : TickM Bool := fun s => ⟨s.count ≤ n, s⟩
-def checkBound' (n : Nat) : Assertion (.arg TickM.State .pure) := fun s => ⌜s.count ≤ n⌝
--- Or if `checkBound'` should be defined without importing `Std.Do`:
--- def checkBound'' (n : Nat) : TickM.State → ULift Prop := fun s => ⟨s.count ≤ n⟩
--- example : checkBound' = checkBound'' := rfl
-
-theorem tick'_spec {Q : PostCond Unit (.arg TickM.State .pure)} :
-    ⦃fun s => Q.1 () ⟨s.count+1⟩⦄ tick' ⦃Q⦄ := by
-  simp [tick', Triple, wp, Id.run]
-
-public theorem checkBound_tick' (n : Nat) :
-    ⦃checkBound' n⦄ tick ⦃⇓ _ => checkBound' (n + 1)⦄ := by
-  set_option trace.Elab.Tactic.Do.vcgen true in
-  -- set_option trace.Debug.Meta.Tactic.simp true in
+private example {P : State → Prop} (h : P ⟨State.count s⟩) :
+    P ⟨State.count s⟩ := by
   set_option trace.Meta.Tactic.simp true in
+  set_option trace.Debug.Meta.Tactic.simp true in
+  set_option trace.Debug.Meta.Tactic.simp.congr true in
   set_option trace.Meta.realizeConst true in
-  -- set_option trace.Debug.Meta.Tactic.simp.congr true in
-  mvcgen [tick]
-  -- Even if I remove the `private` modifier on `count`, I only get as far as
-  -- case vc1
-  -- n : Nat
-  -- ⊢ ∀ (s : State),
-  --   (checkBound' n s).down →
-  --     (wp⟦fun s => ((), { count := s.count + 1 })⟧ (PostCond.noThrow fun x => checkBound' (n + 1)) s).down
-  -- Which `mvcgen` should have "eta-expanded".
+  set_option trace.congr.thm true in
+  simp [*]
 
-end TickM
-end -- public section
+private example {P : State → Prop} (h : P ⟨State.count s⟩) :
+    P ⟨State.count s⟩ := by
+  omega
 
-namespace TickM
-
-end TickM
+private example {P : State → Prop} (h : P ⟨State.count s⟩) :
+    P ⟨State.count s⟩ := by
+  grind
